updates

intermediate2/Zeta.Intermediate.Interleave.fsti
@@ -1,10 +1,19 @@
 module Zeta.Intermediate.Interleave
 
 open FStar.Seq
+open Zeta.SeqAux
 open Zeta.Interleave
 open Zeta.Intermediate.VerifierConfig
+open Zeta.Intermediate.Store
 open Zeta.Intermediate.Verifier
+open Zeta.Intermediate.Logs
 open Zeta.Generic.Interleave
+
+module I = Zeta.Interleave
+module SA = Zeta.SeqAux
+module HI = Zeta.High.Interleave
+module IV = Zeta.Intermediate.Verifier
+module IG = Zeta.Intermediate.Global
 
 let ilog (vcfg: verifier_config) =
   Zeta.Generic.Interleave.ilog (int_verifier_spec vcfg) (vcfg.thread_count)
@@ -23,3 +32,40 @@ let thread_store_pre (#vcfg:_) (tid: nat{tid < vcfg.thread_count}) (il: verifiab
 let thread_store_post (#vcfg:_) (tid: nat{tid < vcfg.thread_count}) (il: verifiable_log vcfg) (i: seq_index il)
   = let vs = thread_state_post tid il i in
     vs.st
+
+let to_logk_entry (#vcfg:_) (il: verifiable_log vcfg) (i: seq_index il)
+  : logK_entry vcfg.app
+  = let gl = to_glog il in
+    let ti = i2s_map il i in
+    IG.to_logk_entry gl ti
+
+let same_shape #a #b #n (il: interleaving a n) (il': interleaving b n)
+  = let ss = s_seq il in
+    let ss' = s_seq il' in
+    (forall (i:SA.seq_index ss). Seq.length (Seq.index ss i) == Seq.length (Seq.index ss i))
+
+val to_logk (#vcfg:_) (il: verifiable_log vcfg)
+  : hil:HI.ilog vcfg.app vcfg.thread_count {same_shape il hil}
+
+val lemma_to_logk_length (#vcfg:_) (il: verifiable_log vcfg)
+  : Lemma (ensures (length il = length (to_logk il)))
+          [SMTPat (to_logk il)]
+
+val lemma_to_logk_src (#vcfg:_) (il: verifiable_log vcfg) (i: seq_index il)
+  : Lemma (ensures src il i == src (to_logk il) i)
+          [SMTPat (src il i)]
+
+val lemma_to_logk_index (#vcfg:_) (ils: verifiable_log vcfg) (i: seq_index ils)
+  : Lemma (ensures (index (to_logk ils) i == to_logk_entry ils i))
+          [SMTPat (index ils i)]
+
+(* every store of every prefix of every thread is a map *)
+val forall_store_ismap (#vcfg:_) (il: verifiable_log vcfg): prop
+
+val elim_forall_store_ismap (#vcfg:_) (il: verifiable_log vcfg) (t:nat{t < vcfg.thread_count})
+  : Lemma (ensures (forall_store_ismap il ==> (let st = thread_store t il in
+                                               is_map st)))
+
+val forall_store_ismap_prefix (#vcfg:_) (il: verifiable_log vcfg) (l:nat{l <= length il})
+  : Lemma (ensures (forall_store_ismap il ==> (let il' = prefix il l in
+                                               forall_store_ismap il')))
