intermediate2/Zeta.Intermediate.TSLog.fsti
@@ -1,11 +1,36 @@
 module Zeta.Intermediate.TSLog
 
+open FStar.Seq
+open Zeta.Interleave
+open Zeta.Generic.Interleave
 open Zeta.Generic.TSLog
 open Zeta.Intermediate.VerifierConfig
 open Zeta.Intermediate.Verifier
 open Zeta.Intermediate.Interleave
 
 module T = Zeta.Generic.TSLog
+module I = Zeta.Interleave
+module HT = Zeta.High.TSLog
 
 let its_log (vcfg:_)
   = T.its_log (int_verifier_spec vcfg) (vcfg.thread_count)
+
+let same_shape #a #b #n (il:I.interleaving a n) (il':I.interleaving b n)
+  = let ss = s_seq il in
+    let ss' = s_seq il' in
+    (forall (i:nat{i < n}). Seq.length (Seq.index ss i) == Seq.length (Seq.index ss i))
+
+val to_logk (#vcfg:_) (il: its_log vcfg)
+  : sil:HT.its_log vcfg.app vcfg.thread_count { same_shape il sil }
+
+val lemma_to_logk_length (#vcfg:_) (il: its_log vcfg)
+  : Lemma (ensures (length il = length (to_logk il)))
+          [SMTPat (to_logk il)]
+
+val lemma_to_logk_prefix_commute (#vcfg:_) (il:its_log vcfg) (i:nat{i <= length il})
+  : Lemma (to_logk (prefix il i) == prefix (to_logk il) i)
+          [SMTPat (prefix il i)]
+
+val lemma_to_logk_src (#vcfg:_) (il: its_log vcfg) (i: seq_index il)
+  : Lemma (ensures (src il i = src (to_logk il) i))
+          [SMTPat (src il i)]
