intermediate2/Zeta.Intermediate.Global.fsti
@@ -1,0 +1,18 @@
+module Zeta.Intermediate.Global
+
+open Zeta.SSeq
+open Zeta.Intermediate.Verifier
+open Zeta.Intermediate.Logs
+open Zeta.Generic.Global
+
+module IT = Zeta.Intermediate.Thread
+
+let verifiable_log (vcfg:_)
+  = Zeta.Generic.Global.verifiable_log (int_verifier_spec vcfg)
+
+let to_logk_entry (#vcfg:_) (gl: verifiable_log vcfg) (i: sseq_index gl)
+  : logK_entry vcfg.app
+  = let t,j = i in
+    let tl = index gl t in
+    IT.to_logk_entry tl j
+
