intermediate2/Zeta.Intermediate.StateRel.fsti
@@ -1,0 +1,137 @@
+module Zeta.Intermediate.StateRel
+
+open Zeta.GenKey
+open Zeta.Intermediate.VerifierConfig
+open Zeta.Intermediate.Store
+open Zeta.Intermediate.Verifier
+open Zeta.Intermediate.Logs
+
+module FE = FStar.FunctionalExtensionality
+module HV = Zeta.High.Verifier
+module GV = Zeta.GenericVerifier
+module Merkle = Zeta.Merkle
+module S = FStar.Seq
+
+(* Relation between thread-local states
+   * either both states have Failed
+   * or both are Valid with equal contents
+     (note that store_rel st st' enforces is_map st) *)
+let vtls_rel #vcfg (vs:vtls_t vcfg) (vs':HV.vtls_t vcfg.app) : Type =
+  vs.valid = vs'.valid /\
+  (vs.valid ==> (vs.tid = vs'.tid /\
+                 vs.clock = vs'.clock /\
+                 store_rel vs.st vs'.st))
+
+let valid_logS_entry (#vcfg:_)
+                     (vs: vtls_t vcfg{vs.valid})
+                     (e: logS_entry _) =
+  let st = vs.st in
+  let s2k = Store.to_slot_state_map st in
+  Logs.valid_logS_entry s2k e
+
+let to_logK_entry (#vcfg:_)
+                  (vs: vtls_t vcfg{vs.valid})
+                  (e: logS_entry _{valid_logS_entry vs e}) =
+  let st = vs.st in
+  let s2k = Store.to_slot_state_map st in
+  Logs.to_logK_entry s2k e
+
+val lemma_runapp_simulates_spec
+      (#vcfg:_)
+      (vs:vtls_t vcfg{vs.valid})
+      (vs':_ {vtls_rel vs vs'})
+      (e:logS_entry vcfg{GV.is_appfn e})
+  : Lemma (requires (valid_logS_entry vs e))
+          (ensures (let ek = to_logK_entry vs e in
+                    vtls_rel (GV.verify_step e vs) (GV.verify_step ek vs')))
+
+(* adding a key not in store to vaddm preserves the spec relationship *)
+val lemma_vaddm_preserves_spec_new_key
+      (#vcfg:_)
+      (vs:vtls_t vcfg{vs.valid})
+      (vs':_ {vtls_rel vs vs'})
+      (e:logS_entry _{GV.AddM? e})
+  : Lemma (requires (let st = vs.st in
+                     let GV.AddM (gk,gv) _  _ = e in
+                     let k = to_base_key gk in
+                     valid_logS_entry vs e /\
+                     not (store_contains_key st k) /\
+                     slot_points_to_is_merkle_points_to st))
+          (ensures (let ek = to_logK_entry vs e in
+                    vtls_rel (GV.verify_step e vs) (GV.verify_step ek vs')))
+
+(* addb preserves spec relationship if the kew is not in store *)
+val lemma_vaddb_preserves_spec_new_key
+      (#vcfg:_)
+      (vs:vtls_t vcfg{vs.valid})
+      (vs':_ {vtls_rel vs vs'})
+      (e:logS_entry _{GV.AddB? e})
+  : Lemma (requires (let st = vs.st in
+                     let GV.AddB (gk,gv) _  _ _ = e in
+                     let k = to_base_key gk in
+                     valid_logS_entry vs e /\
+                     not (store_contains_key st k)))
+          (ensures (let ek = to_logK_entry vs e in
+                    vtls_rel (GV.verify_step e vs) (GV.verify_step ek vs')))
+
+val lemma_evictb_simulates_spec
+      (#vcfg:_)
+      (vs:vtls_t vcfg{vs.valid})
+      (vs':_ {vtls_rel vs vs'})
+      (e:logS_entry vcfg{GV.EvictB? e})
+  : Lemma (requires (let st = vs.st in
+                     valid_logS_entry vs e /\
+                     slot_points_to_is_merkle_points_to st /\
+                     merkle_points_to_uniq st /\
+                     merkle_points_to_desc st))
+          (ensures (let ek = to_logK_entry vs e in
+                    vtls_rel (GV.verify_step e vs) (GV.verify_step ek vs')))
+
+val lemma_evictm_simulates_spec
+      (#vcfg:_)
+      (vs:vtls_t vcfg{vs.valid})
+      (vs':_ {vtls_rel vs vs'})
+      (e:logS_entry vcfg{GV.EvictM? e})
+  : Lemma (requires (let st = vs.st in
+                     vtls_rel vs vs' /\
+                     valid_logS_entry vs e /\
+                     slot_points_to_is_merkle_points_to st /\
+                     merkle_points_to_uniq st /\
+                     merkle_points_to_desc st))
+          (ensures (let ek = to_logK_entry vs e in
+                    vtls_rel (GV.verify_step e vs) (GV.verify_step ek vs')))
+
+val lemma_evictbm_simulates_spec
+      (#vcfg:_)
+      (vs:vtls_t vcfg{vs.valid})
+      (vs':_ {vtls_rel vs vs'})
+      (e:logS_entry vcfg{GV.EvictBM? e})
+  : Lemma (requires (let st = vs.st in
+                     vtls_rel vs vs' /\
+                     valid_logS_entry vs e /\
+                     slot_points_to_is_merkle_points_to st /\
+                     merkle_points_to_uniq st /\
+                     merkle_points_to_desc st))
+          (ensures (let ek = to_logK_entry vs e in
+                    vtls_rel (GV.verify_step e vs) (GV.verify_step ek vs')))
+
+val lemma_nextepoch_simulates_spec
+      (#vcfg:_)
+      (vs:vtls_t vcfg{vs.valid})
+      (vs':_ {vtls_rel vs vs'})
+  : Lemma (requires (vtls_rel vs vs' /\
+                     valid_logS_entry vs GV.NextEpoch))
+          (ensures (let intspec = int_verifier_spec vcfg in
+                    let hispec = HV.high_verifier_spec vcfg.app in
+            vtls_rel #vcfg (GV.verify_step #intspec GV.NextEpoch vs) (GV.verify_step #hispec GV.NextEpoch vs')))
+
+val lemma_verifyepoch_simulates_spec
+      (#vcfg:_)
+      (vs:vtls_t vcfg{vs.valid})
+      (vs':_ {vtls_rel vs vs'})
+  : Lemma (requires (vtls_rel vs vs' /\
+                     valid_logS_entry vs GV.VerifyEpoch))
+          (ensures (let intspec = int_verifier_spec vcfg in
+                    let hispec = HV.high_verifier_spec vcfg.app in
+                    vtls_rel #vcfg (GV.verify_step #intspec GV.VerifyEpoch vs)
+                                   (GV.verify_step #hispec GV.VerifyEpoch vs')))
