intermediate2/Zeta.Intermediate.Thread.fsti
@@ -1,0 +1,23 @@
+module Zeta.Intermediate.Thread
+
+open Zeta.Intermediate.Verifier
+open Zeta.Intermediate.Logs
+open Zeta.Generic.Thread
+
+let verifiable_log (vcfg:_)
+  = Zeta.Generic.Thread.verifiable_log (int_verifier_spec vcfg)
+
+let store (#vcfg:_) (tl: verifiable_log vcfg)
+  = let vs = state tl in
+    vs.st
+
+let store_pre (#vcfg:_) (tl: verifiable_log vcfg) (i: seq_index tl)
+  = let tl' = prefix tl i in
+    store tl'
+
+let store_post (#vcfg:_) (tl: verifiable_log vcfg) (i: seq_index tl)
+  = let tl' = prefix tl (i+1) in
+    store tl'
+
+val to_logk_entry (#vcfg:_) (tl: verifiable_log vcfg) (i: seq_index tl)
+  : logK_entry vcfg.app
